hvhdl/InitializationFacts.v
@@ -1,0 +1,109 @@
+(** * Facts about Initialization *)
+
+Require Import common.Coqlib.
+Require Import common.NatMap.
+
+Require Import hvhdl.Environment.
+Require Import hvhdl.Initialization.
+Require Import hvhdl.AbstractSyntax.
+Require Import hvhdl.SemanticalDomains.
+Require Import hvhdl.Place.
+Require Import hvhdl.HilecopDesignStore.
+Require Import hvhdl.StabilizeFacts.
+
+(** ** Facts about [vruninit] *)
+
+Section VRunInit.
+
+  Lemma vseq_inv_compstore_id :
+        forall {Δ σ Λ flag stmt σ' Λ' id__c σ__c},
+          SSEvaluation.vseq Δ σ Λ flag stmt σ' Λ' ->
+          MapsTo id__c σ__c (compstore σ) ->
+          MapsTo id__c σ__c (compstore σ').
+  Admitted.
+
+  Lemma mapop_inv_compstore_id :
+    forall {Δ Δ__c σ σ__c1 ipmap σ' id__c σ__c2},
+      PortMapEvaluation.mapop Δ Δ__c σ σ__c1 ipmap σ' ->
+      MapsTo id__c σ__c2 (compstore σ) ->
+      MapsTo id__c σ__c2 (compstore σ').
+  Admitted.
+             
+  Lemma vruninit_inv_compstore_id :
+    forall {D__s Δ σ behavior σ' id__c σ__c},
+      vruninit D__s Δ σ behavior σ' ->
+      MapsTo id__c σ__c (compstore σ) ->
+      exists σ__c', MapsTo id__c σ__c' (compstore σ').
+  Proof.
+    induction 1.
+    
+    (* CASE process evaluation *)
+    - exists σ__c; eapply vseq_inv_compstore_id; eauto.
+      
+    (* CASE comp evaluation with events.
+       2 subcases, [id__c = compid] or [id__c ≠ compid] *)
+    - simpl; destruct (Nat.eq_dec compid id__c).
+      + exists σ__c''; rewrite e; apply add_1; auto.
+      + exists σ__c; apply add_2; auto.
+        eapply mapop_inv_compstore_id; eauto.
+
+    (* CASE comp evaluation with no events. *)
+    - exists σ__c; eapply mapop_inv_compstore_id; eauto.
+
+    (* CASE null *)
+    - exists σ__c; assumption.
+
+    (* CASE par *)
+    - unfold IsMergedDState in H2; apply proj2, proj1 in H2.
+      unfold EqualDom in H2; rewrite <- (H2 id__c); exists σ__c; assumption.
+  Qed.
+
+  Lemma vruninit_s_marking_eq_nat :
+    forall Δ σ behavior σ',
+      vruninit hdstore Δ σ behavior σ' ->
+      MapsTo Petri.rst (Vbool false) (sigstore σ) ->
+      forall id__p gm ipm opm σ__p' n,
+        InCs (cs_comp id__p Petri.place_entid gm ipm opm) behavior ->
+        List.In (associp_ ($initial_marking) (e_nat n)) ipm ->
+        NatMap.MapsTo id__p σ__p' (compstore σ') ->
+        NatMap.MapsTo Place.s_marking (Vnat n) (sigstore σ__p').
+  Admitted.
+  
+End VRunInit.
+
+(** ** Facts about [init] *)
+
+Section Init.
+
+  Lemma init_s_marking_eq_nat :
+    forall Δ σ behavior σ0,
+      init hdstore Δ σ behavior σ0 ->
+      forall id__p gm ipm opm σ__p0 n,
+        InCs (cs_comp id__p Petri.place_entid gm ipm opm) behavior ->
+        List.In (associp_ ($initial_marking) (e_nat n)) ipm ->
+        (exists σ__p, MapsTo id__p σ__p (compstore σ)) ->
+        NatMap.MapsTo id__p σ__p0 (compstore σ0) ->
+        NatMap.MapsTo Place.s_marking (Vnat n) (sigstore σ__p0).
+  Proof.
+    inversion 1.
+    intros.
+
+    (* [∃ σ__p s.t. σ(id__p)(rst ← ⊥) = σ__p] *)
+    match goal with
+    | [ ex_MapsTo: exists _, _ , Hvr: vruninit _ _ _ _ _ |- _ ] =>
+      inversion ex_MapsTo as (σ__p, MapsTo_σ__p);
+        specialize (vruninit_inv_compstore_id Hvr MapsTo_σ__p) as ex_MapsTo_σp';
+        inversion ex_MapsTo_σp' as (σ__p', MapsTo_σ__p'); clear ex_MapsTo_σp'
+    end.
+    assert (MapsTo_rst_σ__p' : MapsTo id__p σ__p' (compstore (sstore_add Petri.rst (Vbool true) σ')))
+      by assumption.
+
+    (* [s_marking] value stays the same during stabilization. *)
+    eapply stab_inv_s_marking; eauto.
+
+    (* [s_marking] takes [n] during [vruninit], if [<initial_marking => n>] *)
+    eapply vruninit_s_marking_eq_nat; eauto.
+    simpl; apply add_1; reflexivity.
+  Qed.
+  
+End Init.
