sitpn2hvhdl/GeneratePortsFacts.v
@@ -1,0 +1,140 @@
+(** * Facts about Port Generation and Connection *)
+
+Require Import String.
+Require Import common.StateAndErrorMonad.
+Require Import common.StateAndErrorMonadTactics.
+Require Import common.ListMonadTactics.
+
+Require Import sitpn2hvhdl.Sitpn2HVhdl.
+
+(** ** Facts about Action Port Generation *)
+
+
+Section GenActionPorts.
+  
+  Lemma gen_aports_inv_p2pcomp :
+    forall {sitpn s v s'},
+      generate_action_ports_and_ps sitpn s = OK v s' ->
+      p2pcomp (γ s) = p2pcomp (γ s').
+  Proof.
+    intros *; intros e; minv e; auto; simpl.
+    transitivity (p2pcomp (γ s1)).
+    solve_listm EQ2; intros *; intros e.
+    minv e; solve_listm EQ3.
+    unfold connect_marked_ports in EQ2; solve_listm EQ2.
+    intros *; intros e1; minv e1; solve_listm EQ2.
+    solve_listm EQ0; intros *; intros e; minv e.
+    shelf_state EQ5; change (p2pcomp (γ s)) with (p2pcomp (γ s2)); solve_listm EQ5.
+  Qed.
+
+  Lemma gen_aports_inv_lofPs :
+    forall {sitpn s v s'},
+      generate_action_ports_and_ps sitpn s = OK v s' ->
+      lofPs s = lofPs s'.
+  Proof.
+    intros *; intros e; minv e; auto; simpl.
+    transitivity (lofPs s1).
+    solve_listm EQ2; intros *; intros e.
+    minv e; solve_listm EQ3.
+    unfold connect_marked_ports in EQ2; solve_listm EQ2.
+    intros *; intros e1; minv e1; solve_listm EQ2.
+    solve_listm EQ0; intros *; intros e; minv e.
+    shelf_state EQ5; change (lofPs s) with (lofPs s2); solve_listm EQ5.
+  Qed.
+  
+End GenActionPorts.
+
+(** ** Facts about Function Port Generation *)
+
+Section GenFunPorts.
+
+  Lemma gen_fports_inv_p2pcomp :
+    forall {sitpn s v s'},
+      generate_fun_ports_and_ps sitpn s = OK v s' ->
+      p2pcomp (γ s) = p2pcomp (γ s').
+  Proof.
+    intros *; intros e; minv e; auto.
+    transitivity (p2pcomp (γ s1)).
+    solve_listm EQ2; intros *; intros e; minv e; solve_listm EQ3.
+    unfold connect_fired_ports in EQ2; solve_listm EQ2.
+    intros *; intros e1; minv e1; solve_listm EQ2.
+    solve_listm EQ0; intros *; intros e; minv e.
+    shelf_state EQ5; change (p2pcomp (γ s)) with (p2pcomp (γ s2)); solve_listm EQ5.
+  Qed.
+
+  Lemma gen_fports_inv_lofPs :
+    forall {sitpn s v s'},
+      generate_fun_ports_and_ps sitpn s = OK v s' ->
+      lofPs s = lofPs s'.
+  Proof.
+    intros *; intros e; minv e; auto.
+    transitivity (lofPs s1).
+    solve_listm EQ2; intros *; intros e; minv e; solve_listm EQ3.
+    unfold connect_fired_ports in EQ2; solve_listm EQ2.
+    intros *; intros e1; minv e1; solve_listm EQ2.
+    solve_listm EQ0; intros *; intros e; minv e.
+    shelf_state EQ5; change (lofPs s) with (lofPs s2); solve_listm EQ5.
+  Qed.
+
+  
+End GenFunPorts.
+
+(** ** Facts about Condition Port Generation *)
+
+Section GenCondPorts.
+
+  Lemma gen_cports_inv_p2pcomp :
+    forall {sitpn s v s'},
+      generate_and_connect_cond_ports sitpn s = OK v s' ->
+      p2pcomp (γ s) = p2pcomp (γ s').
+  Proof.
+    intros *; intros e; minv e.
+    solve_listm EQ0.
+    intros *; intros e; minv e.
+    shelf_state EQ5; change (p2pcomp (γ s)) with (p2pcomp (γ s1)).
+    solve_listm EQ5.
+    unfold connect_in_cond_ports in EQ4; solve_listm EQ4.
+    intros *; intros e; minv e; solve_listm EQ1.
+  Qed.
+
+  Lemma gen_cports_inv_lofPs :
+    forall {sitpn s v s'},
+      generate_and_connect_cond_ports sitpn s = OK v s' ->
+      lofPs s = lofPs s'.
+  Proof.
+    intros *; intros e; minv e.
+    solve_listm EQ0.
+    intros *; intros e; minv e.
+    shelf_state EQ5; change (lofPs s) with (lofPs s1).
+    solve_listm EQ5.
+    unfold connect_in_cond_ports in EQ4; solve_listm EQ4.
+    intros *; intros e; minv e; solve_listm EQ1.
+  Qed.
+  
+End GenCondPorts.
+
+(** ** Facts about Port Generation Function *)
+
+Lemma gen_ports_inv_p2pcomp :
+  forall {sitpn s v s'},
+    @generate_ports sitpn s = OK v s' ->
+    p2pcomp (γ s) = p2pcomp (γ s').
+Proof.
+  intros *; intros e; monadInv e.
+  rewrite <- (gen_cports_inv_p2pcomp EQ2),
+  <- (gen_fports_inv_p2pcomp EQ1),
+  <- (gen_aports_inv_p2pcomp EQ);
+    reflexivity.
+Qed.
+
+Lemma gen_ports_inv_lofPs :
+  forall {sitpn s v s'},
+    @generate_ports sitpn s = OK v s' ->
+    lofPs s = lofPs s'.
+Proof.
+  intros *; intros e; monadInv e.
+  rewrite <- (gen_cports_inv_lofPs EQ2),
+  <- (gen_fports_inv_lofPs EQ1),
+  <- (gen_aports_inv_lofPs EQ);
+    reflexivity.
+Qed.
